x86/Asmgen.v
@@ -37,37 +37,58 @@ Definition ireg_of (r: mreg) : res ireg :=
 Definition freg_of (r: mreg) : res freg :=
   match preg_of r with FR mr => OK mr | _ => Error(msg "Asmgen.freg_of") end.
 
+Section WITHINSTRSIZEMAP.
+
+Variable instr_size_map : instruction -> Z.
+Hypothesis instr_size_non_zero : forall i, instr_size_map i > 0.
+
+Definition instr_to_with_info (i: instruction) : instr_with_info :=
+  (i, mk_sizeinfo (instr_size_map i) (instr_size_non_zero i)).
+
+Definition code_to_with_info (c: list instruction) : code :=
+  map instr_to_with_info c.
+
 (** Smart constructors for some operations. *)
 
 Definition mk_mov (rd rs: preg) (k: code) : res code :=
   match rd, rs with
-  | IR rd, IR rs => OK (Pmov_rr rd rs :: k)
-  | FR rd, FR rs => OK (Pmovsd_ff rd rs :: k)
+  | IR rd, IR rs => 
+    OK (instr_to_with_info (Pmov_rr rd rs) :: k)
+  | FR rd, FR rs => 
+    OK (instr_to_with_info (Pmovsd_ff rd rs) :: k)
   | _, _ => Error(msg "Asmgen.mk_mov")
   end.
 
 Definition mk_shrximm (n: int) (k: code) : res code :=
   let p := Int.sub (Int.shl Int.one n) Int.one in
-  OK (Ptestl_rr RAX RAX ::
+  let l := 
+      Ptestl_rr RAX RAX ::
       Pleal RCX (Addrmode (Some RAX) None (inl _ (Int.unsigned p))) ::
       Pcmov Cond_l RAX RCX ::
-      Psarl_ri RAX n :: k).
+      Psarl_ri RAX n :: nil in
+  let c := code_to_with_info l in
+  OK (c ++ k).
 
 Definition mk_shrxlimm (n: int) (k: code) : res code :=
-  OK (if Int.eq n Int.zero then Pmov_rr RAX RAX :: k else
-      Pcqto ::
-      Pshrq_ri RDX (Int.sub (Int.repr 64) n) ::
-      Pleaq RAX (Addrmode (Some RAX) (Some(RDX, 1)) (inl _ 0)) ::
-      Psarq_ri RAX n :: k).
+  let l := 
+      if Int.eq n Int.zero then Pmov_rr RAX RAX :: nil else
+        (Pcqto ::
+         Pshrq_ri RDX (Int.sub (Int.repr 64) n) ::
+         Pleaq RAX (Addrmode (Some RAX) (Some(RDX, 1)) (inl _ 0)) ::
+         Psarq_ri RAX n :: nil) in
+  let c := code_to_with_info l in
+  OK (c ++ k).
 
 Definition low_ireg (r: ireg) : bool :=
   match r with RAX | RBX | RCX | RDX => true | _ => false end.
 
 Definition mk_intconv (mk: ireg -> ireg -> instruction) (rd rs: ireg) (k: code) :=
-  if Archi.ptr64 || low_ireg rs then
-    OK (mk rd rs :: k)
-  else
-    OK (Pmov_rr RAX rs :: mk rd RAX :: k).
+  let l := 
+      if Archi.ptr64 || low_ireg rs then
+        (mk rd rs :: nil)
+      else
+        (Pmov_rr RAX rs :: mk rd RAX :: nil) in
+  OK (code_to_with_info l ++ k).
 
 Definition addressing_mentions (addr: addrmode) (r: ireg) : bool :=
   match addr with Addrmode base displ const =>
@@ -76,43 +97,45 @@ Definition addressing_mentions (addr: addrmode) (r: ireg) : bool :=
   end.
 
 Definition mk_storebyte (addr: addrmode) (rs: ireg) (k: code) :=
-  if Archi.ptr64 || low_ireg rs then
-    OK (Pmovb_mr addr rs :: k)
-  else if addressing_mentions addr RAX then
-    OK (Pleal RCX addr :: Pmov_rr RAX rs ::
-        Pmovb_mr (Addrmode (Some RCX) None (inl _ 0)) RAX :: k)
-  else
-    OK (Pmov_rr RAX rs :: Pmovb_mr addr RAX :: k).
+  let l := 
+      if Archi.ptr64 || low_ireg rs then
+        Pmovb_mr addr rs :: nil
+      else if addressing_mentions addr RAX then
+        Pleal RCX addr :: Pmov_rr RAX rs ::
+        Pmovb_mr (Addrmode (Some RCX) None (inl _ 0)) RAX :: nil
+      else
+        (Pmov_rr RAX rs :: Pmovb_mr addr RAX :: nil) in
+  OK (code_to_with_info l ++ k).
 
 (** Accessing slots in the stack frame. *)
 
 Definition loadind (base: ireg) (ofs: ptrofs) (ty: typ) (dst: mreg) (k: code) :=
   let a := Addrmode (Some base) None (inl _ (Ptrofs.unsigned ofs)) in
   match ty, preg_of dst with
-  | Tint, IR r => OK (Pmovl_rm r a :: k)
-  | Tlong, IR r => OK (Pmovq_rm r a :: k)
-  | Tsingle, FR r => OK (Pmovss_fm r a :: k)
-  | Tsingle, ST0  => OK (Pflds_m a :: k)
-  | Tfloat, FR r => OK (Pmovsd_fm r a :: k)
-  | Tfloat, ST0  => OK (Pfldl_m a :: k)
-  | Tany32, IR r => if Archi.ptr64 then Error (msg "Asmgen.loadind1") else OK (Pmov_rm_a r a :: k)
-  | Tany64, IR r => if Archi.ptr64 then OK (Pmov_rm_a r a :: k) else Error (msg "Asmgen.loadind2")
-  | Tany64, FR r => OK (Pmovsd_fm_a r a :: k)
+  | Tint, IR r => OK (instr_to_with_info (Pmovl_rm r a) ::  k)
+  | Tlong, IR r => OK (instr_to_with_info (Pmovq_rm r a) :: k)
+  | Tsingle, FR r => OK (instr_to_with_info (Pmovss_fm r a) :: k)
+  | Tsingle, ST0  => OK (instr_to_with_info (Pflds_m a) :: k)
+  | Tfloat, FR r => OK (instr_to_with_info (Pmovsd_fm r a) :: k)
+  | Tfloat, ST0  => OK (instr_to_with_info (Pfldl_m a) :: k)
+  | Tany32, IR r => if Archi.ptr64 then Error (msg "Asmgen.loadind1") else OK (instr_to_with_info (Pmov_rm_a r a) :: k)
+  | Tany64, IR r => if Archi.ptr64 then OK (instr_to_with_info (Pmov_rm_a r a) :: k) else Error (msg "Asmgen.loadind2")
+  | Tany64, FR r => OK (instr_to_with_info (Pmovsd_fm_a r a) :: k)
   | _, _ => Error (msg "Asmgen.loadind")
   end.
 
 Definition storeind (src: mreg) (base: ireg) (ofs: ptrofs) (ty: typ) (k: code) :=
   let a := Addrmode (Some base) None (inl _ (Ptrofs.unsigned ofs)) in
   match ty, preg_of src with
-  | Tint, IR r => OK (Pmovl_mr a r :: k)
-  | Tlong, IR r => OK (Pmovq_mr a r :: k)
-  | Tsingle, FR r => OK (Pmovss_mf a r :: k)
-  | Tsingle, ST0 => OK (Pfstps_m a :: k)
-  | Tfloat, FR r => OK (Pmovsd_mf a r :: k)
-  | Tfloat, ST0 => OK (Pfstpl_m a :: k)
-  | Tany32, IR r => if Archi.ptr64 then Error (msg "Asmgen.storeind1") else OK (Pmov_mr_a a r :: k)
-  | Tany64, IR r => if Archi.ptr64 then OK (Pmov_mr_a a r :: k) else Error (msg "Asmgen.storeind2")
-  | Tany64, FR r => OK (Pmovsd_mf_a a r :: k)
+  | Tint, IR r => OK (instr_to_with_info (Pmovl_mr a r) :: k)
+  | Tlong, IR r => OK (instr_to_with_info (Pmovq_mr a r) :: k)
+  | Tsingle, FR r => OK (instr_to_with_info (Pmovss_mf a r) :: k)
+  | Tsingle, ST0 => OK (instr_to_with_info (Pfstps_m a) :: k)
+  | Tfloat, FR r => OK (instr_to_with_info (Pmovsd_mf a r) :: k)
+  | Tfloat, ST0 => OK (instr_to_with_info (Pfstpl_m a) :: k)
+  | Tany32, IR r => if Archi.ptr64 then Error (msg "Asmgen.storeind1") else OK (instr_to_with_info (Pmov_mr_a a r) :: k)
+  | Tany64, IR r => if Archi.ptr64 then OK (instr_to_with_info (Pmov_mr_a a r) :: k) else Error (msg "Asmgen.storeind2")
+  | Tany64, FR r => OK (instr_to_with_info (Pmovsd_mf_a a r) :: k)
   | _, _ => Error (msg "Asmgen.storeind")
   end.
 
@@ -184,35 +207,41 @@ Definition transl_cond
               (cond: condition) (args: list mreg) (k: code) : res code :=
   match cond, args with
   | Ccomp c, a1 :: a2 :: nil =>
-      do r1 <- ireg_of a1; do r2 <- ireg_of a2; OK (Pcmpl_rr r1 r2 :: k)
+      do r1 <- ireg_of a1; do r2 <- ireg_of a2; OK (instr_to_with_info (Pcmpl_rr r1 r2) :: k)
   | Ccompu c, a1 :: a2 :: nil =>
-      do r1 <- ireg_of a1; do r2 <- ireg_of a2; OK (Pcmpl_rr r1 r2 :: k)
+      do r1 <- ireg_of a1; do r2 <- ireg_of a2; OK (instr_to_with_info (Pcmpl_rr r1 r2) :: k)
   | Ccompimm c n, a1 :: nil =>
       do r1 <- ireg_of a1;
-      OK (if Int.eq_dec n Int.zero then Ptestl_rr r1 r1 :: k else Pcmpl_ri r1 n :: k)
+      OK (if Int.eq_dec n Int.zero then 
+            instr_to_with_info (Ptestl_rr r1 r1) :: k 
+          else 
+            instr_to_with_info (Pcmpl_ri r1 n) :: k)
   | Ccompuimm c n, a1 :: nil =>
-      do r1 <- ireg_of a1; OK (Pcmpl_ri r1 n :: k)
+      do r1 <- ireg_of a1; OK (instr_to_with_info (Pcmpl_ri r1 n) :: k)
   | Ccompl c, a1 :: a2 :: nil =>
-      do r1 <- ireg_of a1; do r2 <- ireg_of a2; OK (Pcmpq_rr r1 r2 :: k)
+      do r1 <- ireg_of a1; do r2 <- ireg_of a2; OK (instr_to_with_info (Pcmpq_rr r1 r2) :: k)
   | Ccomplu c, a1 :: a2 :: nil =>
-      do r1 <- ireg_of a1; do r2 <- ireg_of a2; OK (Pcmpq_rr r1 r2 :: k)
+      do r1 <- ireg_of a1; do r2 <- ireg_of a2; OK (instr_to_with_info (Pcmpq_rr r1 r2) :: k)
   | Ccomplimm c n, a1 :: nil =>
       do r1 <- ireg_of a1;
-      OK (if Int64.eq_dec n Int64.zero then Ptestq_rr r1 r1 :: k else Pcmpq_ri r1 n :: k)
+      OK (if Int64.eq_dec n Int64.zero then 
+            instr_to_with_info (Ptestq_rr r1 r1) :: k 
+          else 
+            instr_to_with_info (Pcmpq_ri r1 n) :: k)
   | Ccompluimm c n, a1 :: nil =>
-      do r1 <- ireg_of a1; OK (Pcmpq_ri r1 n :: k)
+      do r1 <- ireg_of a1; OK (instr_to_with_info (Pcmpq_ri r1 n) :: k)
   | Ccompf cmp, a1 :: a2 :: nil =>
-      do r1 <- freg_of a1; do r2 <- freg_of a2; OK (floatcomp cmp r1 r2 :: k)
+      do r1 <- freg_of a1; do r2 <- freg_of a2; OK (instr_to_with_info (floatcomp cmp r1 r2) :: k)
   | Cnotcompf cmp, a1 :: a2 :: nil =>
-      do r1 <- freg_of a1; do r2 <- freg_of a2; OK (floatcomp cmp r1 r2 :: k)
+      do r1 <- freg_of a1; do r2 <- freg_of a2; OK (instr_to_with_info (floatcomp cmp r1 r2) :: k)
   | Ccompfs cmp, a1 :: a2 :: nil =>
-      do r1 <- freg_of a1; do r2 <- freg_of a2; OK (floatcomp32 cmp r1 r2 :: k)
+      do r1 <- freg_of a1; do r2 <- freg_of a2; OK (instr_to_with_info (floatcomp32 cmp r1 r2) :: k)
   | Cnotcompfs cmp, a1 :: a2 :: nil =>
-      do r1 <- freg_of a1; do r2 <- freg_of a2; OK (floatcomp32 cmp r1 r2 :: k)
+      do r1 <- freg_of a1; do r2 <- freg_of a2; OK (instr_to_with_info (floatcomp32 cmp r1 r2) :: k)
   | Cmaskzero n, a1 :: nil =>
-      do r1 <- ireg_of a1; OK (Ptestl_ri r1 n :: k)
+      do r1 <- ireg_of a1; OK (instr_to_with_info (Ptestl_ri r1 n) :: k)
   | Cmasknotzero n, a1 :: nil =>
-      do r1 <- ireg_of a1; OK (Ptestl_ri r1 n :: k)
+      do r1 <- ireg_of a1; OK (instr_to_with_info (Ptestl_ri r1 n) :: k)
   | _, _ =>
      Error(msg "Asmgen.transl_cond")
   end.
@@ -279,30 +308,36 @@ Definition testcond_for_condition (cond: condition) : extcond :=
 (** Acting upon extended conditions. *)
 
 Definition mk_setcc_base (cond: extcond) (rd: ireg) (k: code) :=
-  match cond with
-  | Cond_base c =>
-      Psetcc c rd :: k
-  | Cond_and c1 c2 =>
-      if ireg_eq rd RAX
-      then Psetcc c1 RAX :: Psetcc c2 RCX :: Pandl_rr RAX RCX :: k
-      else Psetcc c1 RAX :: Psetcc c2 rd  :: Pandl_rr rd RAX :: k
-  | Cond_or c1 c2 =>
-      if ireg_eq rd RAX
-      then Psetcc c1 RAX :: Psetcc c2 RCX :: Porl_rr RAX RCX :: k
-      else Psetcc c1 RAX :: Psetcc c2 rd  :: Porl_rr rd RAX :: k
-  end.
+  let l := 
+      match cond with
+      | Cond_base c =>
+        Psetcc c rd :: nil
+      | Cond_and c1 c2 =>
+        if ireg_eq rd RAX
+        then Psetcc c1 RAX :: Psetcc c2 RCX :: Pandl_rr RAX RCX :: nil
+        else Psetcc c1 RAX :: Psetcc c2 rd  :: Pandl_rr rd RAX :: nil
+      | Cond_or c1 c2 =>
+        if ireg_eq rd RAX
+        then Psetcc c1 RAX :: Psetcc c2 RCX :: Porl_rr RAX RCX :: nil
+        else Psetcc c1 RAX :: Psetcc c2 rd  :: Porl_rr rd RAX :: nil
+      end
+  in
+  code_to_with_info l ++ k.
 
 Definition mk_setcc (cond: extcond) (rd: ireg) (k: code) :=
   if Archi.ptr64 || low_ireg rd
   then mk_setcc_base cond rd k
-  else mk_setcc_base cond RAX (Pmov_rr rd RAX :: k).
+  else mk_setcc_base cond RAX (instr_to_with_info (Pmov_rr rd RAX) :: k).
 
 Definition mk_jcc (cond: extcond) (lbl: label) (k: code) :=
-  match cond with
-  | Cond_base c => Pjcc c lbl :: k
-  | Cond_and c1 c2 => Pjcc2 c1 c2 lbl :: k
-  | Cond_or c1 c2 => Pjcc c1 lbl :: Pjcc c2 lbl :: k
-  end.
+  let l :=
+      match cond with
+      | Cond_base c => Pjcc c lbl :: nil
+      | Cond_and c1 c2 => Pjcc2 c1 c2 lbl :: nil
+      | Cond_or c1 c2 => Pjcc c1 lbl :: Pjcc c2 lbl :: nil
+      end
+  in
+  code_to_with_info l ++ k.
 
 (** Translation of the arithmetic operation [r <- op(args)].
   The corresponding instructions are prepended to [k]. *)
@@ -314,208 +349,208 @@ Definition transl_op
       mk_mov (preg_of res) (preg_of a1) k
   | Ointconst n, nil =>
       do r <- ireg_of res;
-      OK ((if Int.eq_dec n Int.zero then Pxorl_r r else Pmovl_ri r n) :: k)
+      OK ((if Int.eq_dec n Int.zero then instr_to_with_info (Pxorl_r r) else instr_to_with_info (Pmovl_ri r n)) :: k)
   | Olongconst n, nil =>
       do r <- ireg_of res;
-      OK ((if Int64.eq_dec n Int64.zero then Pxorq_r r else Pmovq_ri r n) :: k)
+      OK ((if Int64.eq_dec n Int64.zero then instr_to_with_info (Pxorq_r r) else instr_to_with_info (Pmovq_ri r n)) :: k)
   | Ofloatconst f, nil =>
       do r <- freg_of res;
-      OK ((if Float.eq_dec f Float.zero then Pxorpd_f r else Pmovsd_fi r f) :: k)
+      OK ((if Float.eq_dec f Float.zero then instr_to_with_info (Pxorpd_f r) else instr_to_with_info (Pmovsd_fi r f)) :: k)
   | Osingleconst f, nil =>
       do r <- freg_of res;
-      OK ((if Float32.eq_dec f Float32.zero then Pxorps_f r else Pmovss_fi r f) :: k)
+      OK ((if Float32.eq_dec f Float32.zero then instr_to_with_info (Pxorps_f r) else instr_to_with_info (Pmovss_fi r f)) :: k)
   | Oindirectsymbol id, nil =>
       do r <- ireg_of res;
-      OK (Pmov_rs r id :: k)
+      OK (instr_to_with_info (Pmov_rs r id) :: k)
   | Ocast8signed, a1 :: nil =>
       do r1 <- ireg_of a1; do r <- ireg_of res; mk_intconv Pmovsb_rr r r1 k
   | Ocast8unsigned, a1 :: nil =>
       do r1 <- ireg_of a1; do r <- ireg_of res; mk_intconv Pmovzb_rr r r1 k
   | Ocast16signed, a1 :: nil =>
-      do r1 <- ireg_of a1; do r <- ireg_of res; OK (Pmovsw_rr r r1 :: k)
+      do r1 <- ireg_of a1; do r <- ireg_of res; OK (instr_to_with_info (Pmovsw_rr r r1) :: k)
   | Ocast16unsigned, a1 :: nil =>
-      do r1 <- ireg_of a1; do r <- ireg_of res; OK (Pmovzw_rr r r1 :: k)
+      do r1 <- ireg_of a1; do r <- ireg_of res; OK (instr_to_with_info (Pmovzw_rr r r1) :: k)
   | Oneg, a1 :: nil =>
       assertion (mreg_eq a1 res);
-      do r <- ireg_of res; OK (Pnegl r :: k)
+      do r <- ireg_of res; OK (instr_to_with_info (Pnegl r) :: k)
   | Osub, a1 :: a2 :: nil =>
       assertion (mreg_eq a1 res);
-      do r <- ireg_of res; do r2 <- ireg_of a2; OK (Psubl_rr r r2 :: k)
+      do r <- ireg_of res; do r2 <- ireg_of a2; OK (instr_to_with_info (Psubl_rr r r2) :: k)
   | Omul, a1 :: a2 :: nil =>
       assertion (mreg_eq a1 res);
-      do r <- ireg_of res; do r2 <- ireg_of a2; OK (Pimull_rr r r2 :: k)
+      do r <- ireg_of res; do r2 <- ireg_of a2; OK (instr_to_with_info (Pimull_rr r r2) :: k)
   | Omulimm n, a1 :: nil =>
       assertion (mreg_eq a1 res);
-      do r <- ireg_of res; OK (Pimull_ri r n :: k)
+      do r <- ireg_of res; OK (instr_to_with_info (Pimull_ri r n) :: k)
   | Omulhs, a1 :: a2 :: nil =>
       assertion (mreg_eq a1 AX);
       assertion (mreg_eq res DX);
-      do r2 <- ireg_of a2; OK (Pimull_r r2 :: k)
+      do r2 <- ireg_of a2; OK (instr_to_with_info (Pimull_r r2) :: k)
   | Omulhu, a1 :: a2 :: nil =>
       assertion (mreg_eq a1 AX);
       assertion (mreg_eq res DX);
-      do r2 <- ireg_of a2; OK (Pmull_r r2 :: k)
+      do r2 <- ireg_of a2; OK (instr_to_with_info (Pmull_r r2) :: k)
   | Odiv, a1 :: a2 :: nil =>
       assertion (mreg_eq a1 AX);
       assertion (mreg_eq a2 CX);
       assertion (mreg_eq res AX);
-      OK(Pcltd :: Pidivl RCX :: k)
+      OK(instr_to_with_info (Pcltd) :: instr_to_with_info (Pidivl RCX) :: k)
   | Odivu, a1 :: a2 :: nil =>
       assertion (mreg_eq a1 AX);
       assertion (mreg_eq a2 CX);
       assertion (mreg_eq res AX);
-      OK(Pxorl_r RDX :: Pdivl RCX :: k)
+      OK(instr_to_with_info (Pxorl_r RDX) :: instr_to_with_info (Pdivl RCX) :: k)
   | Omod, a1 :: a2 :: nil =>
       assertion (mreg_eq a1 AX);
       assertion (mreg_eq a2 CX);
       assertion (mreg_eq res DX);
-      OK(Pcltd :: Pidivl RCX :: k)
+      OK(instr_to_with_info (Pcltd) :: instr_to_with_info (Pidivl RCX) :: k)
   | Omodu, a1 :: a2 :: nil =>
       assertion (mreg_eq a1 AX);
       assertion (mreg_eq a2 CX);
       assertion (mreg_eq res DX);
-      OK(Pxorl_r RDX :: Pdivl RCX :: k)
+      OK(instr_to_with_info (Pxorl_r RDX) :: instr_to_with_info (Pdivl RCX) :: k)
   | Oand, a1 :: a2 :: nil =>
       assertion (mreg_eq a1 res);
-      do r <- ireg_of res; do r2 <- ireg_of a2; OK (Pandl_rr r r2 :: k)
+      do r <- ireg_of res; do r2 <- ireg_of a2; OK (instr_to_with_info (Pandl_rr r r2) :: k)
   | Oandimm n, a1 :: nil =>
       assertion (mreg_eq a1 res);
-      do r <- ireg_of res; OK (Pandl_ri r n :: k)
+      do r <- ireg_of res; OK (instr_to_with_info (Pandl_ri r n) :: k)
   | Oor, a1 :: a2 :: nil =>
       assertion (mreg_eq a1 res);
-      do r <- ireg_of res; do r2 <- ireg_of a2; OK (Porl_rr r r2 :: k)
+      do r <- ireg_of res; do r2 <- ireg_of a2; OK (instr_to_with_info (Porl_rr r r2) :: k)
   | Oorimm n, a1 :: nil =>
       assertion (mreg_eq a1 res);
-      do r <- ireg_of res; OK (Porl_ri r n :: k)
+      do r <- ireg_of res; OK (instr_to_with_info (Porl_ri r n) :: k)
   | Oxor, a1 :: a2 :: nil =>
       assertion (mreg_eq a1 res);
-      do r <- ireg_of res; do r2 <- ireg_of a2; OK (Pxorl_rr r r2 :: k)
+      do r <- ireg_of res; do r2 <- ireg_of a2; OK (instr_to_with_info (Pxorl_rr r r2) :: k)
   | Oxorimm n, a1 :: nil =>
       assertion (mreg_eq a1 res);
-      do r <- ireg_of res; OK (Pxorl_ri r n :: k)
+      do r <- ireg_of res; OK (instr_to_with_info (Pxorl_ri r n) :: k)
   | Onot, a1 :: nil =>
       assertion (mreg_eq a1 res);
-      do r <- ireg_of res; OK (Pnotl r :: k)
+      do r <- ireg_of res; OK (instr_to_with_info (Pnotl r) :: k)
   | Oshl, a1 :: a2 :: nil =>
       assertion (mreg_eq a1 res);
       assertion (mreg_eq a2 CX);
-      do r <- ireg_of res; OK (Psall_rcl r :: k)
+      do r <- ireg_of res; OK (instr_to_with_info (Psall_rcl r) :: k)
   | Oshlimm n, a1 :: nil =>
       assertion (mreg_eq a1 res);
-      do r <- ireg_of res; OK (Psall_ri r n :: k)
+      do r <- ireg_of res; OK (instr_to_with_info (Psall_ri r n) :: k)
   | Oshr, a1 :: a2 :: nil =>
       assertion (mreg_eq a1 res);
       assertion (mreg_eq a2 CX);
-      do r <- ireg_of res; OK (Psarl_rcl r :: k)
+      do r <- ireg_of res; OK (instr_to_with_info (Psarl_rcl r) :: k)
   | Oshrimm n, a1 :: nil =>
       assertion (mreg_eq a1 res);
-      do r <- ireg_of res; OK (Psarl_ri r n :: k)
+      do r <- ireg_of res; OK (instr_to_with_info (Psarl_ri r n) :: k)
   | Oshru, a1 :: a2 :: nil =>
       assertion (mreg_eq a1 res);
       assertion (mreg_eq a2 CX);
-      do r <- ireg_of res; OK (Pshrl_rcl r :: k)
+      do r <- ireg_of res; OK (instr_to_with_info (Pshrl_rcl r) :: k)
   | Oshruimm n, a1 :: nil =>
       assertion (mreg_eq a1 res);
-      do r <- ireg_of res; OK (Pshrl_ri r n :: k)
+      do r <- ireg_of res; OK (instr_to_with_info (Pshrl_ri r n) :: k)
   | Oshrximm n, a1 :: nil =>
       assertion (mreg_eq a1 AX);
       assertion (mreg_eq res AX);
       mk_shrximm n k
   | Ororimm n, a1 :: nil =>
       assertion (mreg_eq a1 res);
-      do r <- ireg_of res; OK (Prorl_ri r n :: k)
+      do r <- ireg_of res; OK (instr_to_with_info (Prorl_ri r n) :: k)
   | Oshldimm n, a1 :: a2 :: nil =>
       assertion (mreg_eq a1 res);
-      do r <- ireg_of res; do r2 <- ireg_of a2; OK (Pshld_ri r r2 n :: k)
+      do r <- ireg_of res; do r2 <- ireg_of a2; OK (instr_to_with_info (Pshld_ri r r2 n) :: k)
   | Olea addr, _ =>
       do am <- transl_addressing addr args; do r <- ireg_of res;
-      OK (Pleal r (normalize_addrmode_32 am) :: k)
+      OK (instr_to_with_info (Pleal r (normalize_addrmode_32 am)) :: k)
 (* 64-bit integer operations *)
   | Olowlong, a1 :: nil =>
       assertion (mreg_eq a1 res);
-      do r <- ireg_of res; OK (Pmovls_rr r :: k)
+      do r <- ireg_of res; OK (instr_to_with_info (Pmovls_rr r) :: k)
   | Ocast32signed, a1 :: nil =>
-      do r1 <- ireg_of a1; do r <- ireg_of res; OK (Pmovsl_rr r r1 :: k)
+      do r1 <- ireg_of a1; do r <- ireg_of res; OK (instr_to_with_info (Pmovsl_rr r r1) :: k)
   | Ocast32unsigned, a1 :: nil =>
-      do r1 <- ireg_of a1; do r <- ireg_of res; OK (Pmovzl_rr r r1 :: k)
+      do r1 <- ireg_of a1; do r <- ireg_of res; OK (instr_to_with_info (Pmovzl_rr r r1) :: k)
   | Onegl, a1 :: nil =>
       assertion (mreg_eq a1 res);
-      do r <- ireg_of res; OK (Pnegq r :: k)
+      do r <- ireg_of res; OK (instr_to_with_info (Pnegq r) :: k)
   | Oaddlimm n, a1 :: nil =>
       assertion (mreg_eq a1 res);
-      do r <- ireg_of res; OK (Paddq_ri r n :: k)
+      do r <- ireg_of res; OK (instr_to_with_info (Paddq_ri r n) :: k)
   | Osubl, a1 :: a2 :: nil =>
       assertion (mreg_eq a1 res);
-      do r <- ireg_of res; do r2 <- ireg_of a2; OK (Psubq_rr r r2 :: k)
+      do r <- ireg_of res; do r2 <- ireg_of a2; OK (instr_to_with_info (Psubq_rr r r2) :: k)
   | Omull, a1 :: a2 :: nil =>
       assertion (mreg_eq a1 res);
-      do r <- ireg_of res; do r2 <- ireg_of a2; OK (Pimulq_rr r r2 :: k)
+      do r <- ireg_of res; do r2 <- ireg_of a2; OK (instr_to_with_info (Pimulq_rr r r2) :: k)
   | Omullimm n, a1 :: nil =>
       assertion (mreg_eq a1 res);
-      do r <- ireg_of res; OK (Pimulq_ri r n :: k)
+      do r <- ireg_of res; OK (instr_to_with_info (Pimulq_ri r n) :: k)
   | Omullhs, a1 :: a2 :: nil =>
       assertion (mreg_eq a1 AX);
       assertion (mreg_eq res DX);
-      do r2 <- ireg_of a2; OK (Pimulq_r r2 :: k)
+      do r2 <- ireg_of a2; OK (instr_to_with_info (Pimulq_r r2) :: k)
   | Omullhu, a1 :: a2 :: nil =>
       assertion (mreg_eq a1 AX);
       assertion (mreg_eq res DX);
-      do r2 <- ireg_of a2; OK (Pmulq_r r2 :: k)
+      do r2 <- ireg_of a2; OK (instr_to_with_info (Pmulq_r r2) :: k)
   | Odivl, a1 :: a2 :: nil =>
       assertion (mreg_eq a1 AX);
       assertion (mreg_eq a2 CX);
       assertion (mreg_eq res AX);
-      OK(Pcqto :: Pidivq RCX :: k)
+      OK(instr_to_with_info (Pcqto) :: instr_to_with_info (Pidivq RCX) :: k)
   | Odivlu, a1 :: a2 :: nil =>
       assertion (mreg_eq a1 AX);
       assertion (mreg_eq a2 CX);
       assertion (mreg_eq res AX);
-      OK(Pxorq_r RDX :: Pdivq RCX :: k)
+      OK(instr_to_with_info (Pxorq_r RDX) :: instr_to_with_info (Pdivq RCX) :: k)
   | Omodl, a1 :: a2 :: nil =>
       assertion (mreg_eq a1 AX);
       assertion (mreg_eq a2 CX);
       assertion (mreg_eq res DX);
-      OK(Pcqto :: Pidivq RCX :: k)
+      OK(instr_to_with_info (Pcqto) :: instr_to_with_info (Pidivq RCX) :: k)
   | Omodlu, a1 :: a2 :: nil =>
       assertion (mreg_eq a1 AX);
       assertion (mreg_eq a2 CX);
       assertion (mreg_eq res DX);
-      OK(Pxorq_r RDX :: Pdivq RCX :: k)
+      OK(instr_to_with_info (Pxorq_r RDX) :: instr_to_with_info (Pdivq RCX) :: k)
   | Oandl, a1 :: a2 :: nil =>
       assertion (mreg_eq a1 res);
-      do r <- ireg_of res; do r2 <- ireg_of a2; OK (Pandq_rr r r2 :: k)
+      do r <- ireg_of res; do r2 <- ireg_of a2; OK (instr_to_with_info (Pandq_rr r r2) :: k)
   | Oandlimm n, a1 :: nil =>
       assertion (mreg_eq a1 res);
-      do r <- ireg_of res; OK (Pandq_ri r n :: k)
+      do r <- ireg_of res; OK (instr_to_with_info (Pandq_ri r n) :: k)
   | Oorl, a1 :: a2 :: nil =>
       assertion (mreg_eq a1 res);
-      do r <- ireg_of res; do r2 <- ireg_of a2; OK (Porq_rr r r2 :: k)
+      do r <- ireg_of res; do r2 <- ireg_of a2; OK (instr_to_with_info (Porq_rr r r2) :: k)
   | Oorlimm n, a1 :: nil =>
       assertion (mreg_eq a1 res);
-      do r <- ireg_of res; OK (Porq_ri r n :: k)
+      do r <- ireg_of res; OK (instr_to_with_info (Porq_ri r n) :: k)
   | Oxorl, a1 :: a2 :: nil =>
       assertion (mreg_eq a1 res);
-      do r <- ireg_of res; do r2 <- ireg_of a2; OK (Pxorq_rr r r2 :: k)
+      do r <- ireg_of res; do r2 <- ireg_of a2; OK (instr_to_with_info (Pxorq_rr r r2) :: k)
   | Oxorlimm n, a1 :: nil =>
       assertion (mreg_eq a1 res);
-      do r <- ireg_of res; OK (Pxorq_ri r n :: k)
+      do r <- ireg_of res; OK (instr_to_with_info (Pxorq_ri r n) :: k)
   | Onotl, a1 :: nil =>
       assertion (mreg_eq a1 res);
-      do r <- ireg_of res; OK (Pnotq r :: k)
+      do r <- ireg_of res; OK (instr_to_with_info (Pnotq r) :: k)
   | Oshll, a1 :: a2 :: nil =>
       assertion (mreg_eq a1 res);
       assertion (mreg_eq a2 CX);
-      do r <- ireg_of res; OK (Psalq_rcl r :: k)
+      do r <- ireg_of res; OK (instr_to_with_info (Psalq_rcl r) :: k)
   | Oshllimm n, a1 :: nil =>
       assertion (mreg_eq a1 res);
-      do r <- ireg_of res; OK (Psalq_ri r n :: k)
+      do r <- ireg_of res; OK (instr_to_with_info (Psalq_ri r n) :: k)
   | Oshrl, a1 :: a2 :: nil =>
       assertion (mreg_eq a1 res);
       assertion (mreg_eq a2 CX);
-      do r <- ireg_of res; OK (Psarq_rcl r :: k)
+      do r <- ireg_of res; OK (instr_to_with_info (Psarq_rcl r) :: k)
   | Oshrlimm n, a1 :: nil =>
       assertion (mreg_eq a1 res);
-      do r <- ireg_of res; OK (Psarq_ri r n :: k)
+      do r <- ireg_of res; OK (instr_to_with_info (Psarq_ri r n) :: k)
   | Oshrxlimm n, a1 :: nil =>
       assertion (mreg_eq a1 AX);
       assertion (mreg_eq res AX);
@@ -523,76 +558,76 @@ Definition transl_op
   | Oshrlu, a1 :: a2 :: nil =>
       assertion (mreg_eq a1 res);
       assertion (mreg_eq a2 CX);
-      do r <- ireg_of res; OK (Pshrq_rcl r :: k)
+      do r <- ireg_of res; OK (instr_to_with_info (Pshrq_rcl r) :: k)
   | Oshrluimm n, a1 :: nil =>
       assertion (mreg_eq a1 res);
-      do r <- ireg_of res; OK (Pshrq_ri r n :: k)
+      do r <- ireg_of res; OK (instr_to_with_info (Pshrq_ri r n) :: k)
   | Ororlimm n, a1 :: nil =>
       assertion (mreg_eq a1 res);
-      do r <- ireg_of res; OK (Prorq_ri r n :: k)
+      do r <- ireg_of res; OK (instr_to_with_info (Prorq_ri r n) :: k)
   | Oleal addr, _ =>
       do am <- transl_addressing addr args; do r <- ireg_of res;
       OK (match normalize_addrmode_64 am with
-          | (am', None)       => Pleaq r am' :: k
-          | (am', Some delta) => Pleaq r am' :: Paddq_ri r delta :: k
+          | (am', None)       => instr_to_with_info (Pleaq r am') :: k
+          | (am', Some delta) => instr_to_with_info (Pleaq r am') :: instr_to_with_info (Paddq_ri r delta) :: k
           end)
 (**)
   | Onegf, a1 :: nil =>
       assertion (mreg_eq a1 res);
-      do r <- freg_of res; OK (Pnegd r :: k)
+      do r <- freg_of res; OK (instr_to_with_info (Pnegd r) :: k)
   | Oabsf, a1 :: nil =>
       assertion (mreg_eq a1 res);
-      do r <- freg_of res; OK (Pabsd r :: k)
+      do r <- freg_of res; OK (instr_to_with_info (Pabsd r) :: k)
   | Oaddf, a1 :: a2 :: nil =>
       assertion (mreg_eq a1 res);
-      do r <- freg_of res; do r2 <- freg_of a2; OK (Paddd_ff r r2 :: k)
+      do r <- freg_of res; do r2 <- freg_of a2; OK (instr_to_with_info (Paddd_ff r r2) :: k)
   | Osubf, a1 :: a2 :: nil =>
       assertion (mreg_eq a1 res);
-      do r <- freg_of res; do r2 <- freg_of a2; OK (Psubd_ff r r2 :: k)
+      do r <- freg_of res; do r2 <- freg_of a2; OK (instr_to_with_info (Psubd_ff r r2) :: k)
   | Omulf, a1 :: a2 :: nil =>
       assertion (mreg_eq a1 res);
-      do r <- freg_of res; do r2 <- freg_of a2; OK (Pmuld_ff r r2 :: k)
+      do r <- freg_of res; do r2 <- freg_of a2; OK (instr_to_with_info (Pmuld_ff r r2) :: k)
   | Odivf, a1 :: a2 :: nil =>
       assertion (mreg_eq a1 res);
-      do r <- freg_of res; do r2 <- freg_of a2; OK (Pdivd_ff r r2 :: k)
+      do r <- freg_of res; do r2 <- freg_of a2; OK (instr_to_with_info (Pdivd_ff r r2) :: k)
   | Onegfs, a1 :: nil =>
       assertion (mreg_eq a1 res);
-      do r <- freg_of res; OK (Pnegs r :: k)
+      do r <- freg_of res; OK (instr_to_with_info (Pnegs r) :: k)
   | Oabsfs, a1 :: nil =>
       assertion (mreg_eq a1 res);
-      do r <- freg_of res; OK (Pabss r :: k)
+      do r <- freg_of res; OK (instr_to_with_info (Pabss r) :: k)
   | Oaddfs, a1 :: a2 :: nil =>
       assertion (mreg_eq a1 res);
-      do r <- freg_of res; do r2 <- freg_of a2; OK (Padds_ff r r2 :: k)
+      do r <- freg_of res; do r2 <- freg_of a2; OK (instr_to_with_info (Padds_ff r r2) :: k)
   | Osubfs, a1 :: a2 :: nil =>
       assertion (mreg_eq a1 res);
-      do r <- freg_of res; do r2 <- freg_of a2; OK (Psubs_ff r r2 :: k)
+      do r <- freg_of res; do r2 <- freg_of a2; OK (instr_to_with_info (Psubs_ff r r2) :: k)
   | Omulfs, a1 :: a2 :: nil =>
       assertion (mreg_eq a1 res);
-      do r <- freg_of res; do r2 <- freg_of a2; OK (Pmuls_ff r r2 :: k)
+      do r <- freg_of res; do r2 <- freg_of a2; OK (instr_to_with_info (Pmuls_ff r r2) :: k)
   | Odivfs, a1 :: a2 :: nil =>
       assertion (mreg_eq a1 res);
-      do r <- freg_of res; do r2 <- freg_of a2; OK (Pdivs_ff r r2 :: k)
+      do r <- freg_of res; do r2 <- freg_of a2; OK (instr_to_with_info (Pdivs_ff r r2) :: k)
   | Osingleoffloat, a1 :: nil =>
-      do r <- freg_of res; do r1 <- freg_of a1; OK (Pcvtsd2ss_ff r r1 :: k)
+      do r <- freg_of res; do r1 <- freg_of a1; OK (instr_to_with_info (Pcvtsd2ss_ff r r1) :: k)
   | Ofloatofsingle, a1 :: nil =>
-      do r <- freg_of res; do r1 <- freg_of a1; OK (Pcvtss2sd_ff r r1 :: k)
+      do r <- freg_of res; do r1 <- freg_of a1; OK (instr_to_with_info (Pcvtss2sd_ff r r1) :: k)
   | Ointoffloat, a1 :: nil =>
-      do r <- ireg_of res; do r1 <- freg_of a1; OK (Pcvttsd2si_rf r r1 :: k)
+      do r <- ireg_of res; do r1 <- freg_of a1; OK (instr_to_with_info (Pcvttsd2si_rf r r1) :: k)
   | Ofloatofint, a1 :: nil =>
-      do r <- freg_of res; do r1 <- ireg_of a1; OK (Pcvtsi2sd_fr r r1 :: k)
+      do r <- freg_of res; do r1 <- ireg_of a1; OK (instr_to_with_info (Pcvtsi2sd_fr r r1) :: k)
   | Ointofsingle, a1 :: nil =>
-      do r <- ireg_of res; do r1 <- freg_of a1; OK (Pcvttss2si_rf r r1 :: k)
+      do r <- ireg_of res; do r1 <- freg_of a1; OK (instr_to_with_info (Pcvttss2si_rf r r1) :: k)
   | Osingleofint, a1 :: nil =>
-      do r <- freg_of res; do r1 <- ireg_of a1; OK (Pcvtsi2ss_fr r r1 :: k)
+      do r <- freg_of res; do r1 <- ireg_of a1; OK (instr_to_with_info (Pcvtsi2ss_fr r r1) :: k)
   | Olongoffloat, a1 :: nil =>
-      do r <- ireg_of res; do r1 <- freg_of a1; OK (Pcvttsd2sl_rf r r1 :: k)
+      do r <- ireg_of res; do r1 <- freg_of a1; OK (instr_to_with_info (Pcvttsd2sl_rf r r1) :: k)
   | Ofloatoflong, a1 :: nil =>
-      do r <- freg_of res; do r1 <- ireg_of a1; OK (Pcvtsl2sd_fr r r1 :: k)
+      do r <- freg_of res; do r1 <- ireg_of a1; OK (instr_to_with_info (Pcvtsl2sd_fr r r1) :: k)
   | Olongofsingle, a1 :: nil =>
-      do r <- ireg_of res; do r1 <- freg_of a1; OK (Pcvttss2sl_rf r r1 :: k)
+      do r <- ireg_of res; do r1 <- freg_of a1; OK (instr_to_with_info (Pcvttss2sl_rf r r1) :: k)
   | Osingleoflong, a1 :: nil =>
-      do r <- freg_of res; do r1 <- ireg_of a1; OK (Pcvtsl2ss_fr r r1 :: k)
+      do r <- freg_of res; do r1 <- ireg_of a1; OK (instr_to_with_info (Pcvtsl2ss_fr r r1) :: k)
   | Ocmp c, args =>
       do r <- ireg_of res;
       transl_cond c args (mk_setcc (testcond_for_condition c) r k)
@@ -608,21 +643,21 @@ Definition transl_load (chunk: memory_chunk)
   do am <- transl_addressing addr args;
   match chunk with
   | Mint8unsigned =>
-      do r <- ireg_of dest; OK(Pmovzb_rm r am :: k)
+      do r <- ireg_of dest; OK(instr_to_with_info (Pmovzb_rm r am) :: k)
   | Mint8signed =>
-      do r <- ireg_of dest; OK(Pmovsb_rm r am :: k)
+      do r <- ireg_of dest; OK(instr_to_with_info (Pmovsb_rm r am) :: k)
   | Mint16unsigned =>
-      do r <- ireg_of dest; OK(Pmovzw_rm r am :: k)
+      do r <- ireg_of dest; OK(instr_to_with_info (Pmovzw_rm r am) :: k)
   | Mint16signed =>
-      do r <- ireg_of dest; OK(Pmovsw_rm r am :: k)
+      do r <- ireg_of dest; OK(instr_to_with_info (Pmovsw_rm r am) :: k)
   | Mint32 =>
-      do r <- ireg_of dest; OK(Pmovl_rm r am :: k)
+      do r <- ireg_of dest; OK(instr_to_with_info (Pmovl_rm r am) :: k)
   | Mint64 =>
-      do r <- ireg_of dest; OK(Pmovq_rm r am :: k)
+      do r <- ireg_of dest; OK(instr_to_with_info (Pmovq_rm r am) :: k)
   | Mfloat32 =>
-      do r <- freg_of dest; OK(Pmovss_fm r am :: k)
+      do r <- freg_of dest; OK(instr_to_with_info (Pmovss_fm r am) :: k)
   | Mfloat64 =>
-      do r <- freg_of dest; OK(Pmovsd_fm r am :: k)
+      do r <- freg_of dest; OK(instr_to_with_info (Pmovsd_fm r am) :: k)
   | _ =>
       Error (msg "Asmgen.transl_load")
   end.
@@ -635,15 +670,15 @@ Definition transl_store (chunk: memory_chunk)
   | Mint8unsigned | Mint8signed =>
       do r <- ireg_of src; mk_storebyte am r k
   | Mint16unsigned | Mint16signed =>
-      do r <- ireg_of src; OK(Pmovw_mr am r :: k)
+      do r <- ireg_of src; OK(instr_to_with_info (Pmovw_mr am r) :: k)
   | Mint32 =>
-      do r <- ireg_of src; OK(Pmovl_mr am r :: k)
+      do r <- ireg_of src; OK(instr_to_with_info (Pmovl_mr am r) :: k)
   | Mint64 =>
-      do r <- ireg_of src; OK(Pmovq_mr am r :: k)
+      do r <- ireg_of src; OK(instr_to_with_info (Pmovq_mr am r) :: k)
   | Mfloat32 =>
-      do r <- freg_of src; OK(Pmovss_mf am r :: k)
+      do r <- freg_of src; OK(instr_to_with_info (Pmovss_mf am r) :: k)
   | Mfloat64 =>
-      do r <- freg_of src; OK(Pmovsd_mf am r :: k)
+      do r <- freg_of src; OK(instr_to_with_info (Pmovsd_mf am r) :: k)
   | _ =>
       Error (msg "Asmgen.transl_store")
   end.
@@ -670,29 +705,29 @@ Definition transl_instr (f: Mach.function) (i: Mach.instruction)
   | Mstore chunk addr args src =>
       transl_store chunk addr args src k
   | Mcall sig (inl reg) =>
-      do r <- ireg_of reg; OK (Pcall_r r sig :: k)
+      do r <- ireg_of reg; OK (instr_to_with_info (Pcall_r r sig) :: k)
   | Mcall sig (inr symb) =>
-      OK (Pcall_s symb sig :: k)
+      OK (instr_to_with_info (Pcall_s symb sig) :: k)
   | Mtailcall sig (inl reg) =>
       do r <- ireg_of reg;
-      OK (Pfreeframe (StackADT.frame_size (f.(Mach.fn_frame))) f.(fn_retaddr_ofs) f.(fn_link_ofs) ::
-          Pjmp_r r sig :: k)
+      OK (instr_to_with_info (Pfreeframe (StackADT.frame_size (f.(Mach.fn_frame))) f.(fn_retaddr_ofs) f.(fn_link_ofs)) ::
+          instr_to_with_info (Pjmp_r r sig) :: k)
   | Mtailcall sig (inr symb) =>
-      OK (Pfreeframe (StackADT.frame_size (Mach.fn_frame f)) f.(fn_retaddr_ofs) f.(fn_link_ofs) ::
-          Pjmp_s symb sig :: k)
+      OK (instr_to_with_info (Pfreeframe (StackADT.frame_size (Mach.fn_frame f)) f.(fn_retaddr_ofs) f.(fn_link_ofs)) ::
+          instr_to_with_info (Pjmp_s symb sig) :: k)
   | Mlabel lbl =>
-      OK(Plabel lbl :: k)
+      OK(instr_to_with_info (Plabel lbl) :: k)
   | Mgoto lbl =>
-      OK(Pjmp_l lbl :: k)
+      OK(instr_to_with_info (Pjmp_l lbl) :: k)
   | Mcond cond args lbl =>
       transl_cond cond args (mk_jcc (testcond_for_condition cond) lbl k)
   | Mjumptable arg tbl =>
-      do r <- ireg_of arg; OK (Pjmptbl r tbl :: k)
+      do r <- ireg_of arg; OK (instr_to_with_info (Pjmptbl r tbl) :: k)
   | Mreturn =>
-      OK (Pfreeframe (StackADT.frame_size (Mach.fn_frame f)) f.(fn_retaddr_ofs) f.(fn_link_ofs) ::
-          Pret :: k)
+      OK (instr_to_with_info (Pfreeframe (StackADT.frame_size (Mach.fn_frame f)) f.(fn_retaddr_ofs) f.(fn_link_ofs)) ::
+          instr_to_with_info (Pret) :: k)
   | Mbuiltin ef args res =>
-      OK (Pbuiltin ef (List.map (map_builtin_arg preg_of) args) (map_builtin_res preg_of res) :: k)
+      OK (instr_to_with_info (Pbuiltin ef (List.map (map_builtin_arg preg_of) args) (map_builtin_res preg_of res)) :: k)
   end.
 
 (** Translation of a code sequence *)
@@ -738,7 +773,7 @@ Definition transl_code' (f: Mach.function) (il: list Mach.instruction) (axp: boo
 Definition transl_function (f: Mach.function) :=
   do c <- transl_code' f f.(Mach.fn_code) true;
   OK (mkfunction f.(Mach.fn_sig)
-                     (Pallocframe f.(Mach.fn_frame) f.(fn_retaddr_ofs) f.(fn_link_ofs) :: c)
+                     (instr_to_with_info (Pallocframe f.(Mach.fn_frame) f.(fn_retaddr_ofs) f.(fn_link_ofs)) :: c)
                      (f.(Mach.fn_frame))).
 
 Definition transf_function (f: Mach.function) : res Asm.function :=
@@ -753,3 +788,4 @@ Definition transf_fundef (f: Mach.fundef) : res Asm.fundef :=
 Definition transf_program (p: Mach.program) : res Asm.program :=
   transform_partial_program transf_fundef p.
 
+End WITHINSTRSIZEMAP.
